start refactoring

TraceModel.v
@@ -1,4 +1,4 @@
-Require Import Events.
+Require Import Events. 
 Require Import ClassicalExtras.
 Require Import Setoid.
 Require Import List.
@@ -7,76 +7,94 @@ Require Import List.
     in the rest of the development, and prove several results
     about these traces. *)
 
+CoInductive stream {A : Type} :=
+   scons (e : A) (s : stream) : stream. 
 
-(* Inductive endstate : Set := *)
-(* | esgood : endstate *)
-(* | esbad : endstate. *)
-Axiom endstate : Set.
-Axiom an_endstate : endstate.
-
-(** A trace represents either a stopped execution, a silently diverging
-    execution or an infinite execution. *)
-CoInductive trace : Set :=
-  | tstop : endstate -> trace
-  | tsilent : trace
-  | tcons : event -> trace -> trace.
-
-(** A finite prefix is a list of events, that can be continued (ftbd)
-    or not (fstop). *)
-Definition pref := list event.
-
-Inductive finpref : Set :=
-| fstop : pref -> endstate -> finpref
-| ftbd  : pref -> finpref.
-
-Tactic Notation "destruct" "finpref" ident(m) "as" ident(e) ident(f) ident(p) :=
-  destruct m as [ [| e p] f
-                | [| e p]
-                ].
-
-Tactic Notation "induction" "finpref" ident(m) "as" ident(e) ident(f) ident(p) ident(Hp) :=
-  destruct m as [m f | m]; induction m as [|e p Hp].
-
-(** Prefix relation between finite prefixes and traces *)
-(** *prefix relation *)
-Fixpoint fstop_prefix (m : pref) (f : endstate) (t : trace) : Prop :=
-  match m, t with
-    | nil, tstop f' => f = f'
-    | nil, _        => False
-    | cons e1 m', tcons e2 t' => e1 = e2 /\ fstop_prefix m' f t'
-    | _, _          => False
-  end.
-
-Fixpoint ftbd_prefix (m : pref) (t : trace) : Prop :=
-  match m, t with
+Fixpoint list_stream_prefix {A : Type} (l : list A) (s : stream) :=
+  match l, s with
   | nil, _ => True
-  | cons e1 m', tcons e2 t' => e1 = e2 /\ ftbd_prefix m' t'
+  | cons a1 l1, scons a2 s2 => (a1 = a2) /\ (list_stream_prefix l1 s2)
+  end.  
+
+Fixpoint list_list_prefix {A : Type} (l1 l2 : list A) :=
+  match l1, l2 with
+  | nil, _ => True
+  | cons a1 l1, cons a2 l2 => (a1 = a2) /\ list_list_prefix l1 l2
   | _, _ => False
   end.
 
+Lemma list_list_prefix_ref {A : Type} (l : list A) : list_list_prefix l l. 
+Proof. now induction l. Qed. 
+
+Lemma list_list_prefix_trans {A : Type} : forall l1 l2 l3 : list A,
+  list_list_prefix l1 l2 -> list_list_prefix l2 l3 -> list_list_prefix l1 l3.
+Proof.
+  induction l1; try now auto.  
+  intros [] [] H1 H2; inversion H1; inversion H2; subst.
+  simpl. firstorder.
+Qed.
+
+Lemma list_stream_prefix_trans {A : Type} : forall (l1 l2 : list A) (s : stream),
+    list_list_prefix l1 l2 -> list_stream_prefix l2 s ->
+    list_stream_prefix l1 s.
+Proof.
+  induction l1; auto.
+  + intros [] [] Hpref1 Hpref2; inversion Hpref1; inversion Hpref2; subst. 
+    simpl. split; auto; now apply (IHl1 l s).
+Qed.  
+
+(** A trace represents either a stopped execution, a silently diverging
+    execution or an infinite execution. *)
+Variant trace : Set :=
+| tstop (l : list event) (e : endstate) : trace
+| tsilent (l : list event) : trace
+| tstream (s : @stream event) : trace.
+
+(** A finite prefix is a list of events, that can be continued (ftbd)
+    or not (fstop). *)
+Variant finpref : Set :=
+| fstop (l : list event) (es : endstate) : finpref
+| ftbd  (l : list event) : finpref. 
+
+(* Tactic Notation "destruct" "finpref" ident(m) "as" ident(e) ident(f) ident(p) := *)
+(*   destruct m as [ [| e p] f *)
+(*                 | [| e p] *)
+(*                 ]. *)
+
+(* Tactic Notation "induction" "finpref" ident(m) "as" ident(e) ident(f) ident(p) ident(Hp) := *)
+(*   destruct m as [m f | m]; induction m as [|e p Hp]. *)
+
+(** Prefix relation between finite prefixes and traces *)
+(** *prefix relation *)
+
 Definition prefix (m : finpref) (t : trace) : Prop :=
-  match m with
-  | fstop m f => fstop_prefix m f t
-  | ftbd m  => ftbd_prefix m t
-  end.
+  match m, t with
+  | fstop lm em, tstop lt et => em = et /\ lm = lt
+  | ftbd  lm   , tstop lt et => list_list_prefix lm lt
+  | ftbd  lm   , tsilent lt  => list_list_prefix lm lt
+  | ftbd  lm   , tstream s   => list_stream_prefix lm s
+  | _, _ => False
+  end. 
 
 (** Some traces/executions are finite, some are not. *)
 
-Inductive fin : trace -> Prop :=
-  | fin_stop : forall f, fin (tstop f)
-  | fin_cons : forall e t, fin t -> fin (tcons e t).
-
+Definition fin (t : trace) : Prop :=
+  match t with
+  | tstop l f => True
+  | _ => False
+  end. 
+  
 Definition inf (t : trace) : Prop := ~(fin t).
 Hint Unfold inf.
 
 (* A trace is either finite or not *)
 Lemma fin_or_inf : forall t, fin t \/ inf t.
 Proof.
-  intros t. unfold inf. now apply classic.
+ intros t. now apply classic. 
 Qed.
 
-Lemma inf_tcons : forall e t, inf (tcons e t) -> inf t.
-Proof. intros e t H Hc. apply H. now constructor. Qed.
+(* Lemma inf_tcons : forall e t, inf (tcons e t) -> inf t. *)
+(* Proof. intros e t H Hc. apply H. now constructor. Qed. *)
 
 (* A finite prefix has at least two possible continuations
    as we have at least two distinct events
@@ -85,427 +103,413 @@ Proof. intros e t H Hc. apply H. now constructor. Qed.
 Lemma many_continuations :
   forall m ta, inf ta -> exists t', prefix m t' /\ t' <> ta.
 Proof.
-  induction finpref m as e f m IHm; intros ta Hinf.
-  + exists (tstop f). split; try now auto.
-    intros Hc; subst. apply Hinf. now constructor.
-  + destruct ta as [| | e' ta].
-    ++ exfalso. apply Hinf. now constructor.
-    ++ specialize (IHm tsilent Hinf).
-       destruct IHm as [t' [Hpref Hnsilent]].
-       exists (tcons e t'). now split.
-    ++ apply inf_tcons in Hinf. specialize (IHm ta Hinf).
-       destruct IHm as [t' [Hpref Hneq]]. exists (tcons e t').
-       split; try now auto.
-       intros Hc. inversion Hc; now subst.
-  + exists (tstop an_endstate). split; try now auto.
-    intros Hc; subst. apply Hinf. now constructor.
-  + destruct ta as [| | e' ta].
-    ++ exfalso. apply Hinf. now constructor.
-    ++ specialize (IHm tsilent Hinf).
-       destruct IHm as [t' [Hpref Hnsilent]].
-       exists (tcons e t'). now split.
-    ++ apply inf_tcons in Hinf. specialize (IHm ta Hinf).
-       destruct IHm as [t' [Hpref Hneq]]. exists (tcons e t').
-       split; try now auto.
-       intros Hc. inversion Hc; now subst.
+  intros [] t Ht.
+  + destruct t; try now exists (tstop l es).  
+    unfold inf in Ht. exfalso. now apply Ht.   
+  + exists (tstop l an_endstate); split; try now auto. 
+    simpl. now apply list_list_prefix_ref.
+    intros H. rewrite <- H in Ht. unfold inf in Ht.
+    now apply Ht. 
 Qed.
 
 (* We try to identify a finite trace and the fpref made of the same events. *)
 
-Fixpoint fstop_equal (m : pref) (f : endstate) (t : trace) : Prop :=
-  match m, t with
-  | nil, tstop f' => f = f'
-  | cons e1 m', tcons e2 t' => e1 = e2 /\ fstop_equal m' f t'
-  | _, _ => False
-  end.
+(* Fixpoint fstop_equal (m : pref) (f : endstate) (t : trace) : Prop := *)
+(*   match m, t with *)
+(*   | nil, tstop f' => f = f' *)
+(*   | cons e1 m', tcons e2 t' => e1 = e2 /\ fstop_equal m' f t' *)
+(*   | _, _ => False *)
+(*   end. *)
 
-Definition ftbd_equal (m : pref) (t : trace) : Prop := False.
+(* Definition ftbd_equal (m : pref) (t : trace) : Prop := False. *)
 
-Definition equal (m : finpref) (t : trace) : Prop :=
-  match m with
-  | fstop m f => fstop_equal m f t
-  | ftbd m  => ftbd_equal m t
-  end.
-
-Lemma equal_prefix : forall m t, equal m t -> prefix m t.
-Proof.
-  induction finpref m as e f p Hp; destruct t; intros H; simpl in *; now intuition.
-Qed.
-
-Lemma fin_equal : forall t, fin t <-> exists m : finpref, equal m t.
-Proof.
-  intro t. split.
-  - intro H. induction H as [f | e t H [m IH]].
-    + now (exists (fstop nil f)).
-    + destruct m as [m f | m].
-      * now (exists (fstop (cons e m) f)).
-      * now simpl in IH.
-  - intros [m Heq]. generalize dependent t.
-    induction finpref m as e f m' IH; intros t Heq; try now auto.
-    + destruct t; try now auto. now constructor.
-    + destruct t as [| | e' t']; inversion Heq.
-      constructor. now apply IH.
-Qed.
-
-Print prefix.
-Lemma single_cont : forall m t t', equal m t -> prefix m t' -> t = t'.
-Proof.
-  induction finpref m as e f p IHp; destruct t, t'; firstorder;
-  simpl in *; subst.
-  - reflexivity.
-  - now rewrite (IHp t t').
-Qed.
-
-Lemma single_cont_consequence : forall t,
-    fin t -> exists m, forall t', prefix m t' -> t = t'.
-Proof.
-  intros t H. destruct (proj1(fin_equal _) H) as [m H'].
-  exists m. intros t'. now apply single_cont.
-Qed.
-
-(******************************************************************)
-
-(* RB: For now, we do not care about the type of stop. *)
-Fixpoint fstopped (m : finpref) : bool:=
-  match m with
-  | fstop _ _ => true
-  | ftbd  _ => false
-  end. 
-
-(* Fixpoint fisstuck (m : finpref) : bool:= *)
+(* Definition equal (m : finpref) (t : trace) : Prop := *)
 (*   match m with *)
-(*   | fstop _ => false *)
-(*   | fstuck _ => true *)
+(*   | fstop m f => fstop_equal m f t *)
+(*   | ftbd m  => ftbd_equal m t *)
+(*   end. *)
+
+(* Lemma equal_prefix : forall m t, equal m t -> prefix m t. *)
+(* Proof. *)
+(*   induction finpref m as e f p Hp; destruct t; intros H; simpl in *; now intuition. *)
+(* Qed. *)
+
+(* Lemma fin_equal : forall t, fin t <-> exists m : finpref, equal m t. *)
+(* Proof. *)
+(*   intro t. split. *)
+(*   - intro H. induction H as [f | e t H [m IH]]. *)
+(*     + now (exists (fstop nil f)). *)
+(*     + destruct m as [m f | m]. *)
+(*       * now (exists (fstop (cons e m) f)). *)
+(*       * now simpl in IH. *)
+(*   - intros [m Heq]. generalize dependent t. *)
+(*     induction finpref m as e f m' IH; intros t Heq; try now auto. *)
+(*     + destruct t; try now auto. now constructor. *)
+(*     + destruct t as [| | e' t']; inversion Heq. *)
+(*       constructor. now apply IH. *)
+(* Qed. *)
+
+(* Print prefix. *)
+(* Lemma single_cont : forall m t t', equal m t -> prefix m t' -> t = t'. *)
+(* Proof. *)
+(*   induction finpref m as e f p IHp; destruct t, t'; firstorder; *)
+(*   simpl in *; subst. *)
+(*   - reflexivity. *)
+(*   - now rewrite (IHp t t'). *)
+(* Qed. *)
+
+(* Lemma single_cont_consequence : forall t, *)
+(*     fin t -> exists m, forall t', prefix m t' -> t = t'. *)
+(* Proof. *)
+(*   intros t H. destruct (proj1(fin_equal _) H) as [m H']. *)
+(*   exists m. intros t'. now apply single_cont. *)
+(* Qed. *)
+
+(* (******************************************************************) *)
+
+(* (* RB: For now, we do not care about the type of stop. *) *)
+(* Fixpoint fstopped (m : finpref) : bool:= *)
+(*   match m with *)
+(*   | fstop _ _ => true *)
 (*   | ftbd  _ => false *)
 (*   end.  *)
 
-Lemma stop_single_continuation : forall m t1 t2,
-    fstopped m = true ->
-    prefix m t1 -> prefix m t2 ->
-    t1 = t2.
-Proof.
-  intros [m | m]; induction m; intros [] [] H H0 H1; try now auto.
-  + simpl in *. now subst.
-  + inversion H0. inversion H1. clear H0 H1.
-    subst. simpl in H. specialize (IHm t t0 H H3 H5).
-    now subst.
-Qed.
+(* (* Fixpoint fisstuck (m : finpref) : bool:= *) *)
+(* (*   match m with *) *)
+(* (*   | fstop _ => false *) *)
+(* (*   | fstuck _ => true *) *)
+(* (*   | ftbd  _ => false *) *)
+(* (*   end.  *) *)
 
-(* Lemma stuck_sngle_continuation : forall m t1 t2, *)
-(*     fisstuck m = true -> *)
+(* Lemma stop_single_continuation : forall m t1 t2, *)
+(*     fstopped m = true -> *)
 (*     prefix m t1 -> prefix m t2 -> *)
 (*     t1 = t2. *)
 (* Proof. *)
-(*   intros [m | m | m]; induction m; intros [] [] H H0 H1; try now auto. *)
+(*   intros [m | m]; induction m; intros [] [] H H0 H1; try now auto. *)
+(*   + simpl in *. now subst. *)
 (*   + inversion H0. inversion H1. clear H0 H1. *)
 (*     subst. simpl in H. specialize (IHm t t0 H H3 H5). *)
 (*     now subst. *)
 (* Qed. *)
 
-Lemma equal_stopped : forall m t,
-    equal m t ->
-    fstopped m = true.
-Proof.
-  intros [m | m]; induction m; intros t H;
-  try now auto.
-Qed.
+(* (* Lemma stuck_sngle_continuation : forall m t1 t2, *) *)
+(* (*     fisstuck m = true -> *) *)
+(* (*     prefix m t1 -> prefix m t2 -> *) *)
+(* (*     t1 = t2. *) *)
+(* (* Proof. *) *)
+(* (*   intros [m | m | m]; induction m; intros [] [] H H0 H1; try now auto. *) *)
+(* (*   + inversion H0. inversion H1. clear H0 H1. *) *)
+(* (*     subst. simpl in H. specialize (IHm t t0 H H3 H5). *) *)
+(* (*     now subst. *) *)
+(* (* Qed. *) *)
 
-(************************************************************************)
+(* Lemma equal_stopped : forall m t, *)
+(*     equal m t -> *)
+(*     fstopped m = true. *)
+(* Proof. *)
+(*   intros [m | m]; induction m; intros t H; *)
+(*   try now auto. *)
+(* Qed. *)
 
-CoFixpoint constant_trace (e : event) : trace := tcons e (constant_trace e).
+(* (************************************************************************) *)
 
-Theorem trace_eta : forall t, t = match t with
-                                  | tstop f => tstop f
-                                  | tsilent => tsilent
-                                  | tcons e t' => tcons e t'
-                                  end.
-Proof. destruct t; reflexivity. Qed.
 
-Lemma constant_trace_eta : forall e, constant_trace e = tcons e (constant_trace e).
-Proof. intro e. now rewrite trace_eta at 1. Qed.
+CoFixpoint constant_stream (e : event) : stream := scons e (constant_stream e).
 
-Lemma inf_constant_trace :  forall e, inf (constant_trace e).
-Proof.
-  intros e Hc. remember (constant_trace e).
-  induction Hc; rewrite constant_trace_eta in Heqt;
-  now inversion Heqt.
-Qed.
+(* Theorem trace_eta : forall t, t = match t with *)
+(*                                   | tstop f => tstop f *)
+(*                                   | tsilent => tsilent *)
+(*                                   | tcons e t' => tcons e t' *)
+(*                                   end. *)
+(* Proof. destruct t; reflexivity. Qed. *)
 
-Lemma const_not_fin : forall e, ~ (exists t, fin t /\ constant_trace e = t).
-Proof.
-  intros e [t [Ht Heq]].
-  rewrite <- Heq in Ht. now apply (inf_constant_trace e Ht).
-Qed.
+(* Lemma constant_trace_eta : forall e, constant_trace e = tcons e (constant_trace e). *)
+(* Proof. intro e. now rewrite trace_eta at 1. Qed. *)
 
-CoInductive all (e:event) : trace -> Prop :=
-| acons : forall t, all e t -> all e (tcons e t).
+(* Lemma inf_constant_trace :  forall e, inf (constant_trace e). *)
+(* Proof. *)
+(*   intros e Hc. remember (constant_trace e). *)
+(*   induction Hc; rewrite constant_trace_eta in Heqt; *)
+(*   now inversion Heqt. *)
+(* Qed. *)
 
-(* RB: This may be extended with the end state later. *)
-Inductive ends_with (e:event) : trace -> Prop :=
-| eall : forall t, all e t -> ends_with e t
-| egrow : forall t e', ends_with e t -> ends_with e (tcons e' t).
+(* Lemma const_not_fin : forall e, ~ (exists t, fin t /\ constant_trace e = t). *)
+(* Proof. *)
+(*   intros e [t [Ht Heq]]. *)
+(*   rewrite <- Heq in Ht. now apply (inf_constant_trace e Ht). *)
+(* Qed. *)
 
-Lemma ends_with_different : forall t,
-  ends_with an_event t -> ends_with another_event t -> False.
-Proof.
-   intros t Ha Hb. induction Ha.
-  - induction Hb.
-    + inversion H; inversion H0; subst.
-      pose proof different_events. congruence.
-    + now inversion H; subst.
-  - inversion Hb; subst.
-    + inversion H; subst. apply IHHa. now constructor.
-    + easy.
-Qed.
+(* CoInductive all (e:event) : trace -> Prop := *)
+(* | acons : forall t, all e t -> all e (tcons e t). *)
 
-(************************************************************************)
+(* (* RB: This may be extended with the end state later. *) *)
+(* Inductive ends_with (e:event) : trace -> Prop := *)
+(* | eall : forall t, all e t -> ends_with e t *)
+(* | egrow : forall t e', ends_with e t -> ends_with e (tcons e' t). *)
 
-(** *embed *)
-(* a way to get a trace t from a finite prefix m is
-   to consider the trace made of the same events of m
-   and then add a tstop.
- *)
+(* Lemma ends_with_different : forall t, *)
+(*   ends_with an_event t -> ends_with another_event t -> False. *)
+(* Proof. *)
+(*    intros t Ha Hb. induction Ha. *)
+(*   - induction Hb. *)
+(*     + inversion H; inversion H0; subst. *)
+(*       pose proof different_events. congruence. *)
+(*     + now inversion H; subst. *)
+(*   - inversion Hb; subst. *)
+(*     + inversion H; subst. apply IHHa. now constructor. *)
+(*     + easy. *)
+(* Qed. *)
 
-(* RB: What to do with the final state? For now, we leave it as before. *)
-Fixpoint embedding_pref (m : pref) (term : trace) : trace :=
+(* (************************************************************************) *)
+
+(* (** *embed *) *)
+(* (* a way to get a trace t from a finite prefix m is *)
+(*    to consider the trace made of the same events of m *)
+(*    and then add a tstop. *)
+(*  *) *)
+
+(* (* RB: What to do with the final state? For now, we leave it as before. *) *)
+(* Fixpoint embedding_pref (m : pref) (term : trace) : trace := *)
+(*   match m with *)
+(*   | nil => term *)
+(*   | cons e m' => tcons e (embedding_pref m' term) *)
+(*   end. *)
+
+(* Section Embedding. *)
+
+(* Variable es : endstate. *)
+
+Definition embedding (es : endstate) (m : finpref) : trace :=
   match m with
-  | nil => term
-  | cons e m' => tcons e (embedding_pref m' term)
+  | fstop l f => tstop l f
+  | ftbd l => tstop l es
   end.
 
-Section Embedding.
+Lemma embed_pref (es : endstate) : forall m, prefix m (embedding es m).
+Proof. destruct m; simpl; auto; apply list_list_prefix_ref. Qed.
 
-Variable es : endstate.
+(* Lemma embed_fin : forall m, fin (embedding m). *)
+(* Proof. now destruct m. Qed. *)
 
-Definition embedding (m : finpref) : trace :=
-  match m with
-  | fstop m f => embedding_pref m (tstop f)
-  | ftbd m => embedding_pref m (tstop es)
-  end.
+(* Lemma embed_eq : forall m, fstopped m = true -> equal m (embedding m). *)
+(* Proof. destruct m as [m | m]; induction m; intros H; try now auto. *)
+(*        simpl in *. now auto. *)
+(* Qed. *)
 
-Lemma embed_pref : forall m, prefix m (embedding m).
-Proof. destruct m as [m | m]; now induction m. Qed.
+(* Lemma equal_embedding : forall m t, *)
+(*     equal m t -> *)
+(*     embedding m = t. *)
+(* Proof. *)
+(*   destruct m as [m | m]; induction m; intros t Heq; destruct t; try now auto. *)
+(*   - inversion Heq. simpl. now subst. *)
+(*   - inversion Heq. simpl. subst. *)
+(*     assert (H: equal (fstop m e) t) by auto. *)
+(*     assert (H': (embedding (fstop m e)) = embedding_pref m (tstop e)) by auto. *)
+(*     specialize (IHm t H). now subst. *)
+(* Qed. *)
 
-Lemma embed_fin : forall m, fin (embedding m).
-Proof. destruct m as [m | m]; induction m; now constructor. Qed. 
+(* Lemma embed_cons:  forall m t e, *)
+(*     embedding m = t -> *)
+(*     (tcons e (embedding m)) = tcons e t. *)
+(* Proof. *)
+(*   intros [] t a He; try now destruct t. *)
+(*   simpl in *. now rewrite He. *)
+(*   simpl in *. now rewrite He. *)
+(* Qed. *)
 
-Lemma embed_eq : forall m, fstopped m = true -> equal m (embedding m).
-Proof. destruct m as [m | m]; induction m; intros H; try now auto.
-       simpl in *. now auto.
-Qed.
+(* End Embedding. *)
 
-Lemma equal_embedding : forall m t,
-    equal m t ->
-    embedding m = t.
-Proof.
-  destruct m as [m | m]; induction m; intros t Heq; destruct t; try now auto.
-  - inversion Heq. simpl. now subst.
-  - inversion Heq. simpl. subst.
-    assert (H: equal (fstop m e) t) by auto.
-    assert (H': (embedding (fstop m e)) = embedding_pref m (tstop e)) by auto.
-    specialize (IHm t H). now subst.
-Qed.
+(* (************************************************************************) *)
 
-Lemma embed_cons:  forall m t e,
-    embedding m = t ->
-    (tcons e (embedding m)) = tcons e t.
-Proof.
-  intros [] t a He; try now destruct t.
-  simpl in *. now rewrite He.
-  simpl in *. now rewrite He.
-Qed.
-
-End Embedding.
-
-(************************************************************************)
-
-(** The relation fpr is the prefix relation between two prefixes *)
+(* (** The relation fpr is the prefix relation between two prefixes *) *)
 
 
-(* CA: we can define a prefix relation among finite prefixes *)
+(* (* CA: we can define a prefix relation among finite prefixes *) *)
 
-Fixpoint fpr_ftbd (m1 m2 : pref) : Prop :=
+(* Fixpoint fpr_ftbd (m1 m2 : pref) : Prop := *)
+(*   match m1, m2 with *)
+(*   | nil, _ => True *)
+(*   | cons e1 m1', cons e2 m2' => e1 = e2 /\ fpr_ftbd m1' m2' *)
+(*   | _, _ => False *)
+(*   end. *)
+
+(* (* Not used!! *) *)
+(* Fixpoint fpr_fstop (m1 m2 : pref) : Prop := *)
+(*   match m1, m2 with *)
+(*   | nil, nil => True *)
+(*   | cons e1 m1', cons e2 m2' => e1 = e2 /\ fpr_fstop m1' m2' *)
+(*   | _, _ => False *)
+(*   end. *)
+
+Definition fpr (m1 m2 : finpref) : Prop :=
   match m1, m2 with
-  | nil, _ => True
-  | cons e1 m1', cons e2 m2' => e1 = e2 /\ fpr_ftbd m1' m2'
+  | ftbd l1, ftbd l2 => list_list_prefix l1 l2
+  | ftbd l1, fstop l2 e2 => list_list_prefix l1 l2
+  | fstop l1 e1, fstop l2 e2 => e1 = e2 /\ l1 = l2
   | _, _ => False
-  end.
+  end. 
 
-(* Not used!! *)
-Fixpoint fpr_fstop (m1 m2 : pref) : Prop :=
-  match m1, m2 with
-  | nil, nil => True
-  | cons e1 m1', cons e2 m2' => e1 = e2 /\ fpr_fstop m1' m2'
-  | _, _ => False
-  end.
+(* Fixpoint fpr (m1 m2 : finpref) : Prop := *)
+(*   match m1, m2 with *)
+(*   | ftbd m1, ftbd m2 | ftbd m1, fstop m2 _ => fpr_ftbd m1 m2 *)
+(*   (* | ftbd m1, fstop m2 => fpr_ftbd m1 m2 *)                                  *)
+(*   | fstop m1 f1, fstop m2 f2 => m1 = m2 /\ f1 = f2 (* or fpr_fstop m1 m2 *) *)
+(*   | fstop m1 f1, ftbd m2 => False *)
+(*   end. *)
 
-Fixpoint fpr (m1 m2 : finpref) : Prop :=
-  match m1, m2 with
-  | ftbd m1, ftbd m2 | ftbd m1, fstop m2 _ => fpr_ftbd m1 m2
-  (* | ftbd m1, fstop m2 => fpr_ftbd m1 m2 *)                                 
-  | fstop m1 f1, fstop m2 f2 => m1 = m2 /\ f1 = f2 (* or fpr_fstop m1 m2 *)
-  | fstop m1 f1, ftbd m2 => False
-  end.
+(* Lemma fpr_reflexivity : forall m, fpr m m. *)
+(* Proof.  destruct m as [m | m]; now induction m. Qed. *)
 
-Lemma fpr_reflexivity : forall m, fpr m m.
-Proof.  destruct m as [m | m]; now induction m. Qed.
+(* Lemma fpr_transitivity : forall m1 m2 m3, *)
+(*     fpr m1 m2 -> fpr m2 m3 -> fpr m1 m3. *)
+(* Proof. *)
+(*   destruct m1 as [m1 | m1]; *)
+(*   induction m1; intros [m2 | m2] [m3 | m3] H2 H3; auto; *)
+(*   destruct m2; inversion H2; auto; *)
+(*     destruct m3; inversion H3; subst; simpl; try discriminate; try split; auto. *)
+(*   - inversion H; subst. inversion H1; subst. reflexivity. *)
+(*   - inversion H1; subst. reflexivity. *)
+(*   - apply (IHm1 (ftbd m2) (ftbd m3)); [easy |]. *)
+(*     simpl in *. inversion H1; subst. now pose proof fpr_reflexivity (ftbd m3). *)
+(*   - now apply (IHm1 (ftbd m2) (ftbd m3)). *)
+(*   - now apply (IHm1 (ftbd m2) (ftbd m3)). *)
+(* Qed. *)
 
-Lemma fpr_transitivity : forall m1 m2 m3,
-    fpr m1 m2 -> fpr m2 m3 -> fpr m1 m3.
-Proof.
-  destruct m1 as [m1 | m1];
-  induction m1; intros [m2 | m2] [m3 | m3] H2 H3; auto;
-  destruct m2; inversion H2; auto;
-    destruct m3; inversion H3; subst; simpl; try discriminate; try split; auto.
-  - inversion H; subst. inversion H1; subst. reflexivity.
-  - inversion H1; subst. reflexivity.
-  - apply (IHm1 (ftbd m2) (ftbd m3)); [easy |].
-    simpl in *. inversion H1; subst. now pose proof fpr_reflexivity (ftbd m3).
-  - now apply (IHm1 (ftbd m2) (ftbd m3)).
-  - now apply (IHm1 (ftbd m2) (ftbd m3)).
-Qed.
-
-Lemma fpr_antisymmetry : forall (m m' : finpref),
-    fpr m m' /\ fpr m' m -> m = m'.
-Proof.
-  intros m.
-  induction finpref m as e f p IHp;
-    intros m' [H1 H2];
-    destruct finpref m' as e' f' p';
-    try now auto.
-  - inversion H1. now subst.
-  - now inversion H1.
-  - now inversion H1.
-  - specialize (IHp (ftbd p')).
-    inversion H1 as [Heq Hpp']; inversion H2 as [_ Hp'p].
-    subst.
-    simpl in IHp. assert (H: fpr_ftbd p p' /\ fpr_ftbd p' p).
-    {
-      inversion Heq; subst.
-      now pose proof fpr_reflexivity (ftbd p').
-    }
-    now inversion Heq.
-  - specialize (IHp (ftbd p')).
-    destruct H1 as [Heq Hpp']; destruct H2 as [_ Hp'p].
-    subst.
-    assert (H: fpr_ftbd p p' /\ fpr_ftbd p' p) by auto.
-    specialize (IHp H). now inversion IHp.
-Qed.
+(* Lemma fpr_antisymmetry : forall (m m' : finpref), *)
+(*     fpr m m' /\ fpr m' m -> m = m'. *)
+(* Proof. *)
+(*   intros m. *)
+(*   induction finpref m as e f p IHp; *)
+(*     intros m' [H1 H2]; *)
+(*     destruct finpref m' as e' f' p'; *)
+(*     try now auto. *)
+(*   - inversion H1. now subst. *)
+(*   - now inversion H1. *)
+(*   - now inversion H1. *)
+(*   - specialize (IHp (ftbd p')). *)
+(*     inversion H1 as [Heq Hpp']; inversion H2 as [_ Hp'p]. *)
+(*     subst. *)
+(*     simpl in IHp. assert (H: fpr_ftbd p p' /\ fpr_ftbd p' p). *)
+(*     { *)
+(*       inversion Heq; subst. *)
+(*       now pose proof fpr_reflexivity (ftbd p'). *)
+(*     } *)
+(*     now inversion Heq. *)
+(*   - specialize (IHp (ftbd p')). *)
+(*     destruct H1 as [Heq Hpp']; destruct H2 as [_ Hp'p]. *)
+(*     subst. *)
+(*     assert (H: fpr_ftbd p p' /\ fpr_ftbd p' p) by auto. *)
+(*     specialize (IHp H). now inversion IHp. *)
+(* Qed. *)
 
 
 Lemma fpr_pref_pref : forall m1 m2 t,
     fpr m1 m2 -> prefix m2 t -> prefix m1 t.
 Proof.
-  destruct m1 as [m1 | m1].
-  - induction m1; intros [] [] H1 H2;
-      try destruct H1 as [H1 H1']; try destruct H2 as [H2 H2'];
-      simpl in *; subst; try (now auto).
-  - induction m1 as [| e m1'].
-    + intros [] [] H1 H2; simpl in *;
-        try destruct H1 as []; try destruct H2 as [H2 H2'];
-        subst; try (now auto).
-    + intros m2 t. intros H1 H2.
-      destruct m2 as [[| e2 m2'] f | [| e2 m2']]; simpl in *; subst; try (now auto);
-        destruct H1; subst; destruct t; try contradiction;
-        destruct H2; subst; split; auto.
-      * specialize (IHm1' (fstop m2' f) t); simpl in *; auto.
-      * specialize (IHm1' (ftbd m2') t); simpl in *; auto.
+  intros [] [] [] Hfpr Hpref; try now auto; simpl in *; (try firstorder; now subst).  
+  + simpl in *. now apply (list_list_prefix_trans l l0 l1).
+  + simpl in *. now apply (list_list_prefix_trans l l0 l1).
+  + simpl in *. now apply (list_stream_prefix_trans l l0 s). 
 Qed.
 
-Lemma a_foo_lemma : forall m,
-    fpr m (ftbd nil) -> m = ftbd nil.
-Proof. destruct m as [m | m]; now induction m. Qed.
+(* Lemma a_foo_lemma : forall m, *)
+(*     fpr m (ftbd nil) -> m = ftbd nil. *)
+(* Proof. destruct m as [m | m]; now induction m. Qed. *)
 
-(* Lemma another_foo_lemma : forall m1 m2 e, *)
-(*     fpr m1 m2 -> fpr (fcons e m1) (fcons e m2). *)
-(* Proof. destruct m as [m1 | m1]; now induction m1. Qed. *)
+(* (* Lemma another_foo_lemma : forall m1 m2 e, *) *)
+(* (*     fpr m1 m2 -> fpr (fcons e m1) (fcons e m2). *) *)
+(* (* Proof. destruct m as [m1 | m1]; now induction m1. Qed. *) *)
 
+Lemma list_list_same_ext : forall (l1 l2 l : list event),
+    list_list_prefix l1 l -> list_list_prefix l2 l ->
+    (list_list_prefix l1 l2 \/ list_list_prefix l2 l1). 
+Proof.
+  induction l1.
+  + now left.
+  + intros [] [] Hpref1 Hpref2; try now right. 
+    ++ inversion Hpref1; inversion Hpref2; subst; simpl.
+       destruct (IHl1 l l0); now auto.
+Qed.      
+
+Lemma list_stream_same_ext : forall (l1 l2 : list event) (s : stream),
+    list_stream_prefix l1 s -> list_stream_prefix l2 s ->
+    (list_list_prefix l1 l2 \/ list_list_prefix l2 l1).
+Proof.
+  induction l1.
+  + now left.
+  + intros [] [] Hpref1 Hpref2.
+    ++ now right.
+    ++ inversion Hpref1; inversion Hpref2; subst; simpl.
+       destruct (IHl1 l s); now auto.
+Qed.
+                               
+  
 Lemma same_ext : forall m1 m2 t,
     prefix m1 t -> prefix m2 t ->
     fpr m1 m2 \/ fpr m2 m1.
 Proof.
-  destruct m1 as [m1 | m1]; induction m1; intros [] [] H1 H2;
-    try (now auto); destruct H1; destruct p; simpl in *;
-      destruct H2; simpl in *; subst; try (now auto);
-    try specialize (IHm1 _ _ H0);
-    try (specialize (IHm1 (fstop p e0) t H0 H2); simpl in IHm1;
-    destruct IHm1 as [IHm1 | IHm1]; destruct IHm1; subst;
-    [now left | now right]);
-    try (specialize (IHm1 (ftbd p) t H0 H2); simpl in IHm1;
-    destruct IHm1; subst;
-    [now left | now right]).
-  - specialize (IHm1 (fstop p e) t H0 H2); simpl in IHm1;
-    destruct IHm1 as [IHm1 | IHm1]; subst;
-    [now left | now right].
-Qed.
+  intros m1 m2 [] Hpref1 Hpref2.
+  + destruct m1, m2; simpl in *.
+    ++ inversion Hpref1; inversion Hpref2; subst; now auto.
+    ++ inversion Hpref1; subst; now right.
+    ++ inversion Hpref2; subst; now left.
+    ++ now apply (list_list_same_ext l0 l1 l).
+  + destruct m1, m2; simpl in *.
+    ++ inversion Hpref1; inversion Hpref2; subst; now auto.
+    ++ inversion Hpref1; subst; now right.
+    ++ inversion Hpref2; subst; now left.
+    ++ now apply (list_list_same_ext l0 l1 l).
+  +  destruct m1, m2; simpl in *.
+    ++ inversion Hpref1; inversion Hpref2; subst; now auto.
+    ++ inversion Hpref1; subst; now right.
+    ++ inversion Hpref2; subst; now left.
+    ++ now apply (list_stream_same_ext l l0 s).
+Qed.   
 
 Lemma same_fpr : forall m1 m2 m,
     fpr m1 m -> fpr m2 m ->
     (fpr m1 m2 \/ fpr m2 m1).
 Proof.
-  destruct m1 as [p1 | p1]; destruct m2 as [p2 | p2]; destruct m as [p | p];
-    try now auto.
-  - generalize dependent p2. generalize dependent p.
-    induction p1.
-    + intros p p2 H1 H2; try destruct H1; try destruct H2; simpl in *; subst; now left.
-    + intros p p2 H1 H2; try destruct H1; try destruct H2; simpl in *; subst; now left.
-  - generalize dependent p2. generalize dependent p.
-    induction p1.
-    + intros p p2 H1 H2; try destruct H1; try destruct H2; simpl in *; subst; now right.
-    + intros p p2 H1 H2; try destruct H1; try destruct H2; simpl in *; subst; now right.
-  - generalize dependent p2. generalize dependent p.
-    induction p1.
-    + intros p p2 H1 H2; try destruct H1; try destruct H2; simpl in *; subst; now left.
-    + intros p p2 H1 H2; try destruct H1; try destruct H2; simpl in *; subst; now left.
-  - generalize dependent p2. generalize dependent p.
-    induction p1.
-    + intros p p2 H1 H2. simpl in *; subst; now left.
-    + intros p p2 H1 H2. simpl in *; subst.
-      destruct p as [| a' p'].
-      ++ contradiction.
-      ++ destruct H1; subst. destruct p2; auto.
-         simpl in H2; destruct H2; subst. specialize (IHp1 p' p2 H0 H1).
-         destruct IHp1; [now left | now right].
-  - generalize dependent p2. generalize dependent p.
-    induction p1.
-    + intros p p2 H1 H2. simpl in *; subst; now left.
-    + intros p p2 H1 H2. simpl in *; subst.
-      destruct p as [| a' p'].
-      ++ contradiction.
-      ++ destruct H1; subst. destruct p2; auto.
-         simpl in H2; destruct H2; subst. specialize (IHp1 p' p2 H0 H1).
-         destruct IHp1; [now left | now right].
-Qed.
+  intros [] [] [] Hpref1 Hpref2; simpl in Hpref1, Hpref2; try now auto. 
+  + inversion Hpref1; inversion Hpref2; subst. now auto.
+  + inversion Hpref1; subst. now right.
+  + inversion Hpref2; subst. now left.
+  + simpl. now apply (list_list_same_ext l l0 l1).
+  + simpl. now apply (list_list_same_ext l l0 l1).
+Qed. 
+  
 
-Lemma non_comp_pref_diff_traces : forall t1 t2 m1 m2,
-    prefix m1 t1 -> prefix m2 t2 ->
-    ~ (fpr m1 m2 \/ fpr m2 m1) -> t1 <> t2.
-Proof.
-  intros t1 t2 m1 m2 H H0 H1 Hf.
-  subst. apply H1. now apply (same_ext m1 m2 t2).
-Qed.
+(* Lemma non_comp_pref_diff_traces : forall t1 t2 m1 m2, *)
+(*     prefix m1 t1 -> prefix m2 t2 -> *)
+(*     ~ (fpr m1 m2 \/ fpr m2 m1) -> t1 <> t2. *)
+(* Proof. *)
+(*   intros t1 t2 m1 m2 H H0 H1 Hf. *)
+(*   subst. apply H1. now apply (same_ext m1 m2 t2). *)
+(* Qed. *)
 
-Lemma no_prper_fpr_ftbd : forall m, m <> ftbd nil -> fpr m (ftbd nil) -> False.
-Proof. destruct m as [m | m]; now induction m. Qed.
+(* Lemma no_prper_fpr_ftbd : forall m, m <> ftbd nil -> fpr m (ftbd nil) -> False. *)
+(* Proof. destruct m as [m | m]; now induction m. Qed. *)
 
-Lemma stop_sngle_continuation_fpr : forall m1 m2,
-    fstopped m1 = true ->
-    fpr m1 m2 ->
-    m1 = m2.
-Proof.
-  destruct m1 as [m1 | m1]; destruct m2 as [m2 | m2];
-    induction m1, m2;
-    intros H H0;
-    inversion H0; subst;
-    try now auto.
-  - congruence.
-Qed.
+(* Lemma stop_sngle_continuation_fpr : forall m1 m2, *)
+(*     fstopped m1 = true -> *)
+(*     fpr m1 m2 -> *)
+(*     m1 = m2. *)
+(* Proof. *)
+(*   destruct m1 as [m1 | m1]; destruct m2 as [m2 | m2]; *)
+(*     induction m1, m2; *)
+(*     intros H H0; *)
+(*     inversion H0; subst; *)
+(*     try now auto. *)
+(*   - congruence. *)
+(* Qed. *)
 
-(**************************************************)
+(* (**************************************************) *)
 
-(** *snoc *)
+(* (** *snoc *) *)
 
-(* CA: fsnoc is the identity on fstop *)
+
+(* (* CA: fsnoc is the identity on fstop *) *)
 
 Fixpoint snoc {A : Type} (l : list A) (x : A) : list A :=
   match l with
@@ -513,468 +517,474 @@ Fixpoint snoc {A : Type} (l : list A) (x : A) : list A :=
   | cons x' l' => cons x' (snoc l' x)
   end.
 
-Definition fsnoc (m : finpref) (e : event) :=
-  match m with
-  | fstop m' _ => m
-  | ftbd  m' => ftbd (snoc m' e)
-  end.
+(* Definition fsnoc (m : finpref) (e : event) := *)
+(*   match m with *)
+(*   | fstop m' _ => m *)
+(*   | ftbd  m' => ftbd (snoc m' e) *)
+(*   end. *)
 
-Lemma stop_snoc_id : forall m e,
-    fstopped m = true ->
-    fsnoc m e = m.
+(* Lemma stop_snoc_id : forall m e, *)
+(*     fstopped m = true -> *)
+(*     fsnoc m e = m. *)
+(* Proof. *)
+(*   induction m; try now auto. *)
+(* Qed. *)
+
+Lemma list_prefix_snoc_list_prefix {A : Type} : forall (l1 l2 : list A) (a : A),
+    list_list_prefix l1 l2 ->
+    list_list_prefix l1 (snoc l2 a).
 Proof.
-  induction m; try now auto.
+  induction l1.
+  + auto.
+  + destruct l2. contradiction.
+    intros a1 H1. inversion H1; subst. 
+    simpl. split; auto; now apply (IHl1 l2 a0). 
 Qed.
 
-Lemma fpr_snoc_fpr : forall m1 m2 e,
-    fpr m1 m2 ->
-    fpr m1 (fsnoc m2 e).
-Proof.
-  destruct m1 as [m1 | m1]; induction m1; intros [] e' H; try now auto;
-  inversion H; subst.
-  + simpl in *. destruct p. contradiction.
-    destruct H as [H1 H2].
-    specialize (IHm1 (ftbd p) e' H2). now split.
-Qed.
-
-Lemma snoc_stop' : forall m e b, fstopped (fsnoc m e) = b ->
-                            fstopped m = b.
-Proof.
-  intros m e b H. now destruct m.
-Qed.
+(* Lemma snoc_stop' : forall m e b, fstopped (fsnoc m e) = b -> *)
+(*                             fstopped m = b. *)
+(* Proof. *)
+(*   intros m e b H. now destruct m. *)
+(* Qed. *)
 
 
-Lemma snoc_stop : forall m e b, fstopped (fsnoc m e) = b <->
-                                fstopped m = b.
-Proof.
-  intros m e b. split.
-  - now apply snoc_stop'.
-  - intros H. apply NNPP. intros ff.
-    destruct (fstopped (fsnoc m e)) eqn : Heq;
-    destruct b;  try (now apply ff);
-    apply snoc_stop' in Heq; now rewrite H in Heq.
-Qed.
+(* Lemma snoc_stop : forall m e b, fstopped (fsnoc m e) = b <-> *)
+(*                                 fstopped m = b. *)
+(* Proof. *)
+(*   intros m e b. split. *)
+(*   - now apply snoc_stop'. *)
+(*   - intros H. apply NNPP. intros ff. *)
+(*     destruct (fstopped (fsnoc m e)) eqn : Heq; *)
+(*     destruct b;  try (now apply ff); *)
+(*     apply snoc_stop' in Heq; now rewrite H in Heq. *)
+(* Qed. *)
 
 
-Lemma compare_with_snoc : forall m1 m e,
-    fpr m1 (fsnoc m e) ->
-    (fpr m1 m \/ m1 = fsnoc m e).
-Proof.
-  destruct m1 as [m1 | m1]; induction m1; destruct m as [m | m];
-    induction m; intros e' H; try now auto.
-  + inversion H. assert (fpr (ftbd m1) (ftbd nil)).
-    { auto. }
-    apply a_foo_lemma in H2.
-    subst; simpl. inversion H2; now right.
-  + simpl in *.
-    destruct H. subst; simpl in *.
-    specialize (IHm1 (ftbd m) e' H0). simpl in *. destruct IHm1.
-    ++ now left.
-    ++ right. inversion H. now subst.
-Qed.
+(* Lemma compare_with_snoc : forall m1 m e, *)
+(*     fpr m1 (fsnoc m e) -> *)
+(*     (fpr m1 m \/ m1 = fsnoc m e). *)
+(* Proof. *)
+(*   destruct m1 as [m1 | m1]; induction m1; destruct m as [m | m]; *)
+(*     induction m; intros e' H; try now auto. *)
+(*   + inversion H. assert (fpr (ftbd m1) (ftbd nil)). *)
+(*     { auto. } *)
+(*     apply a_foo_lemma in H2. *)
+(*     subst; simpl. inversion H2; now right. *)
+(*   + simpl in *. *)
+(*     destruct H. subst; simpl in *. *)
+(*     specialize (IHm1 (ftbd m) e' H0). simpl in *. destruct IHm1. *)
+(*     ++ now left. *)
+(*     ++ right. inversion H. now subst. *)
+(* Qed. *)
 
-Lemma snoc_diff : forall m a b,
-    fstopped m = false ->
-    fpr (fsnoc m a) (fsnoc m b) ->
-    a = b.
-Proof.
-  intros [m|m] a b H H0; [now inversion H |].
-  clear H. simpl in *.
-  eapply (compare_with_snoc (fsnoc (ftbd m) a) (ftbd m) b) in H0.
-  destruct H0 as [H0 | H0]; auto.
-  - induction m; inversion H0; auto; try now apply IHm.
-  - induction m; inversion H0; auto.
-    assert (H: fsnoc (ftbd m) a = fsnoc (ftbd m) b).
-    { simpl. now rewrite H1. }
-    now specialize (IHm H).
-Qed.
+(* Lemma snoc_diff : forall m a b, *)
+(*     fstopped m = false -> *)
+(*     fpr (fsnoc m a) (fsnoc m b) -> *)
+(*     a = b. *)
+(* Proof. *)
+(*   intros [m|m] a b H H0; [now inversion H |]. *)
+(*   clear H. simpl in *. *)
+(*   eapply (compare_with_snoc (fsnoc (ftbd m) a) (ftbd m) b) in H0. *)
+(*   destruct H0 as [H0 | H0]; auto. *)
+(*   - induction m; inversion H0; auto; try now apply IHm. *)
+(*   - induction m; inversion H0; auto. *)
+(*     assert (H: fsnoc (ftbd m) a = fsnoc (ftbd m) b). *)
+(*     { simpl. now rewrite H1. } *)
+(*     now specialize (IHm H). *)
+(* Qed. *)
 
-Lemma no_snoc_fpr_ftb : forall m e, ~ fpr (fsnoc m e) (ftbd nil).
-Proof. destruct m as [m | m]; now induction m. Qed.
+(* Lemma no_snoc_fpr_ftb : forall m e, ~ fpr (fsnoc m e) (ftbd nil). *)
+(* Proof. destruct m as [m | m]; now induction m. Qed. *)
 
-Lemma fpr_snoc_ftbd : forall m e f,
-    fstopped m = false ->
-    fpr (fsnoc m e) (fsnoc (ftbd nil) f) ->
-    m = ftbd nil.
-Proof.
-  intros [m|m] e' f H H0; [now induction m |].
-  + apply compare_with_snoc in H0. destruct H0.
-    now apply no_snoc_fpr_ftb in H0.
-    simpl in H0. inversion H0.
-    destruct m; auto.
-    simpl in *. clear H. inversion H2. subst.
-    assert (H: ~ (snoc m e' = nil)).
-    { now induction m. }
-    contradiction.
-Qed.
+(* Lemma fpr_snoc_ftbd : forall m e f, *)
+(*     fstopped m = false -> *)
+(*     fpr (fsnoc m e) (fsnoc (ftbd nil) f) -> *)
+(*     m = ftbd nil. *)
+(* Proof. *)
+(*   intros [m|m] e' f H H0; [now induction m |]. *)
+(*   + apply compare_with_snoc in H0. destruct H0. *)
+(*     now apply no_snoc_fpr_ftb in H0. *)
+(*     simpl in H0. inversion H0. *)
+(*     destruct m; auto. *)
+(*     simpl in *. clear H. inversion H2. subst. *)
+(*     assert (H: ~ (snoc m e' = nil)). *)
+(*     { now induction m. } *)
+(*     contradiction. *)
+(* Qed. *)
 
-Lemma same_snoc_same_finpref : forall m m0 e1 e2 i1 i2,
-    i1 <> i2  -> e1 <> e2 ->
-    fstopped m0 = false ->
-    fstopped m = false ->
-    fpr (fsnoc m0 i1) (fsnoc m e1) ->
-    fpr (fsnoc m0 i2) (fsnoc m e2) ->
-    m0 = m.
-Proof.
-  destruct m as [m | m]; induction m as [| e' m' IHm'];
-  intros m0 e1 e2 i1 i2 H H0 H1 H2 H3 H4;
-  try now auto; simpl in *.
-  + now apply (fpr_snoc_ftbd m0 i1 e1).
-  + destruct m0 as [m0 | m0];
-    [now inversion H1 |].
-    destruct m0 as [| e0 m0]; simpl in *. destruct H3, H4; subst; contradiction.
-    destruct H3, H4; subst.
-    specialize (IHm' (ftbd m0) e1 e2 i1 i2 H H0 H1 H2 H5 H6). now inversion IHm'.
-Qed.
+(* Lemma same_snoc_same_finpref : forall m m0 e1 e2 i1 i2, *)
+(*     i1 <> i2  -> e1 <> e2 -> *)
+(*     fstopped m0 = false -> *)
+(*     fstopped m = false -> *)
+(*     fpr (fsnoc m0 i1) (fsnoc m e1) -> *)
+(*     fpr (fsnoc m0 i2) (fsnoc m e2) -> *)
+(*     m0 = m. *)
+(* Proof. *)
+(*   destruct m as [m | m]; induction m as [| e' m' IHm']; *)
+(*   intros m0 e1 e2 i1 i2 H H0 H1 H2 H3 H4; *)
+(*   try now auto; simpl in *. *)
+(*   + now apply (fpr_snoc_ftbd m0 i1 e1). *)
+(*   + destruct m0 as [m0 | m0]; *)
+(*     [now inversion H1 |]. *)
+(*     destruct m0 as [| e0 m0]; simpl in *. destruct H3, H4; subst; contradiction. *)
+(*     destruct H3, H4; subst. *)
+(*     specialize (IHm' (ftbd m0) e1 e2 i1 i2 H H0 H1 H2 H5 H6). now inversion IHm'. *)
+(* Qed. *)
 
-Lemma snoc_lemma : forall m,
-    m = ftbd nil \/
-    (exists m' e', m = fsnoc m' e').
-Proof.
-  intros [m f | m]; induction m.
-  - right. now exists (fstop nil f), an_event.
-  - destruct IHm as [H | H]; try now inversion H.
-    right. destruct H as [m' [e' H]]. now exists (fstop (cons a m) f), e'.
-  - now left.
-  - destruct IHm as [H | H]. 
-    + inversion H; subst. right. now exists (ftbd nil), a.
-    + destruct H as [m' [e' H]]. right.
-      destruct m' as [m' | m'].
-      now exists (ftbd (cons a m')), e'.
-      inversion H. exists (ftbd (cons a m')), e'. now subst. 
-Qed.
+(* Lemma snoc_lemma : forall m, *)
+(*     m = ftbd nil \/ *)
+(*     (exists m' e', m = fsnoc m' e'). *)
+(* Proof. *)
+(*   intros [m f | m]; induction m. *)
+(*   - right. now exists (fstop nil f), an_event. *)
+(*   - destruct IHm as [H | H]; try now inversion H. *)
+(*     right. destruct H as [m' [e' H]]. now exists (fstop (cons a m) f), e'. *)
+(*   - now left. *)
+(*   - destruct IHm as [H | H].  *)
+(*     + inversion H; subst. right. now exists (ftbd nil), a. *)
+(*     + destruct H as [m' [e' H]]. right. *)
+(*       destruct m' as [m' | m']. *)
+(*       now exists (ftbd (cons a m')), e'. *)
+(*       inversion H. exists (ftbd (cons a m')), e'. now subst.  *)
+(* Qed. *)
 
-Lemma not_stop_not_snoc_pref : forall m e,
-    fstopped m = false ->
-    fpr (fsnoc m e) m -> False.
-Proof.
-  intros [m f | m] e H H0; induction m; try now auto.
-  simpl in *. destruct H0 as [Heq H0].
-  apply IHm; try reflexivity. assumption.
-Qed.
+(* Lemma not_stop_not_snoc_pref : forall m e, *)
+(*     fstopped m = false -> *)
+(*     fpr (fsnoc m e) m -> False. *)
+(* Proof. *)
+(*   intros [m f | m] e H H0; induction m; try now auto. *)
+(*   simpl in *. destruct H0 as [Heq H0]. *)
+(*   apply IHm; try reflexivity. assumption. *)
+(* Qed. *)
 
-Lemma snoc_m_event_equal : forall m e1 e2,
-    fstopped m = false ->
-    fpr (fsnoc m e1) (fsnoc m e2) ->
-    e1 = e2.
-Proof.
-  intros [m f | m] e1 e2 Hstop Hfpr;
-  induction m; inversion Hfpr; try now auto.
-Qed.
+(* Lemma snoc_m_event_equal : forall m e1 e2, *)
+(*     fstopped m = false -> *)
+(*     fpr (fsnoc m e1) (fsnoc m e2) -> *)
+(*     e1 = e2. *)
+(* Proof. *)
+(*   intros [m f | m] e1 e2 Hstop Hfpr; *)
+(*   induction m; inversion Hfpr; try now auto. *)
+(* Qed. *)
 
-Lemma same_snoc_same_pointwise : forall m1 m2 e1 e2,
-    fstopped m1 = false ->
-    fstopped m2 = false ->
-    fsnoc m1 e1 = fsnoc m2 e2 ->
-    m1 = m2 /\ e1 = e2.
-Proof.
-  destruct m1 as [m1 | m1]; induction m1; intros m2 e1 e2 Hstop1 Hstop2 Heq;
-    try now auto.
-  + destruct m2 as [m2 | m2]; destruct m2; inversion Heq; try now auto.
-    simpl in *. 
-    ++ now destruct m2. 
-  + destruct m2 as [m2 | m2]; destruct m2; inversion Heq; try now auto.
-    ++ exfalso. apply (no_snoc_fpr_ftb (ftbd m1) e1). simpl in *. now rewrite H1. 
-    ++ destruct (IHm1 (ftbd m2) e1 e2); simpl in *; subst; try now auto.
-       now rewrite H1. inversion H; now subst.
-Qed.
+(* Lemma same_snoc_same_pointwise : forall m1 m2 e1 e2, *)
+(*     fstopped m1 = false -> *)
+(*     fstopped m2 = false -> *)
+(*     fsnoc m1 e1 = fsnoc m2 e2 -> *)
+(*     m1 = m2 /\ e1 = e2. *)
+(* Proof. *)
+(*   destruct m1 as [m1 | m1]; induction m1; intros m2 e1 e2 Hstop1 Hstop2 Heq; *)
+(*     try now auto. *)
+(*   + destruct m2 as [m2 | m2]; destruct m2; inversion Heq; try now auto. *)
+(*     simpl in *.  *)
+(*     ++ now destruct m2.  *)
+(*   + destruct m2 as [m2 | m2]; destruct m2; inversion Heq; try now auto. *)
+(*     ++ exfalso. apply (no_snoc_fpr_ftb (ftbd m1) e1). simpl in *. now rewrite H1.  *)
+(*     ++ destruct (IHm1 (ftbd m2) e1 e2); simpl in *; subst; try now auto. *)
+(*        now rewrite H1. inversion H; now subst. *)
+(* Qed. *)
 
-(* TODO: TM#2 *)
-Inductive diverges : trace -> Prop :=
-| div_silent : diverges tsilent
-| div_cons : forall e t, diverges t -> diverges (tcons e t).
+(* (* TODO: TM#2 *) *)
 
+Definition diverges (t : trace) : Prop :=
+  match t with
+  | tsilent l => True
+  | _ => False
+  end. 
+
+(* Inductive diverges : trace -> Prop := *)
+(* | div_silent : diverges tsilent *)
+(* | div_cons : forall e t, diverges t -> diverges (tcons e t). *)
+
+(* (* Lemma proper_prefix : forall m t, *) *)
+(* (*     prefix m t -> *) *)
+(* (*     embedding m <> t -> *) *)
+(* (*     fstopped m = false -> *) *)
+(* (*     (exists e, prefix (fsnoc m e) t). *) *)
 (* Lemma proper_prefix : forall m t, *)
 (*     prefix m t -> *)
-(*     embedding m <> t -> *)
+(*     (forall es, embedding es m <> t) -> *)
 (*     fstopped m = false -> *)
+(*     ~ diverges t -> *)
 (*     (exists e, prefix (fsnoc m e) t). *)
-Lemma proper_prefix : forall m t,
-    prefix m t ->
-    (forall es, embedding es m <> t) ->
-    fstopped m = false ->
-    ~ diverges t ->
-    (exists e, prefix (fsnoc m e) t).
+(* Proof. *)
+(*   Print diverges. *)
+(*   destruct m as [m f| m]; induction m; intros t Hpref Hembed Hstop Hdiv; try now auto. *)
+(*   + destruct t. *)
+(*     * specialize (Hembed e). contradiction. *)
+(*     * now pose proof div_silent. *)
+(*     * now exists e. *)
+(*   + destruct t; try now auto. *)
+(*     inversion Hpref. subst. destruct (IHm t) as [e' h]; try now auto. *)
+(*     * intros ff. specialize (Hembed ff). *)
+(*       intros Hembed'. *)
+(*       pose proof embed_cons ff (ftbd m) t e as Hcontra. specialize (Hcontra Hembed'). *)
+(*       now apply Hembed. *)
+(*     * intros ff. now pose proof div_cons e t ff. *)
+(*     * now exists e'. *)
+(* Qed. *)
+
+(* Lemma fpr_stop_equal : forall m1 m2, *)
+(*     fpr m1 m2 -> *)
+(*     fstopped m1 = true -> *)
+(*     m1 = m2. *)
+(* Proof. *)
+(*   intros [m1 | m1]; induction m1; intros [m2 | m2] Hpref Hstop; *)
+(*     try easy; *)
+(*     inversion Hpref; congruence. *)
+(* Qed. *)
+
+
+(* (**********************************************************************) *)
+
+(* (** *m[fstop/ftbd] *) *)
+
+(* Section Embedding'. *)
+
+(* Variable es : endstate. *)
+
+(* Definition same_events_with_stop (m : finpref) : finpref := *)
+(*   match m with *)
+(*   | ftbd m => fstop m es *)
+(*   | fstop m f => fstop m f *)
+(*   end. *)
+
+(* Lemma with_stop_fstopped : forall m, *)
+(*     fstopped (same_events_with_stop m) = true. *)
+(* Proof. destruct m; auto. Qed. *)
+
+(* Lemma if_fstopped_equal : forall m, *)
+(*     fstopped m = true -> *)
+(*     m = same_events_with_stop m. *)
+(* Proof. *)
+(*   now destruct m. *)
+(* Qed. *)
+
+(* Lemma embedding_is_the_same : forall m, *)
+(*     embedding es m = *)
+(*     embedding es (same_events_with_stop m). *)
+(* Proof. *)
+(*   intros m. destruct m; try easy. *)
+(* Qed. *)
+
+(* Lemma m_fpr_with_stop : forall m, *)
+(*     fpr m (same_events_with_stop m). *)
+(* Proof. destruct m as [m | m]; now induction m. Qed. *)
+
+(* Lemma with_stop_prefix_embedding :forall m, *)
+(*     prefix (same_events_with_stop m) (embedding es m). *)
+(* Proof. destruct m as [m | m]; now induction m. Qed. *)
+
+(* Lemma equal_with_stop_same_embedding : forall m mm, *)
+(*     fstopped m = true -> *)
+(*     fpr mm m -> *)
+(*     fpr m (same_events_with_stop mm) -> *)
+(*     embedding es m = embedding es mm. *)
+(* Proof. *)
+(*   destruct m as [m | m]; destruct m; *)
+(*     intros mm Hstop Hfpr HfprStop; try now destruct mm. *)
+(*   simpl in *.  *)
+(*   destruct mm; try now auto; simpl in *. inversion Hfpr; subst. reflexivity. *)
+(*   destruct HfprStop; simpl in *; now subst. *)
+(*   destruct mm as [mm | mm]; simpl in *; *)
+(*     try destruct Hfpr; try destruct HfprStop; now subst. *)
+(* Qed. *)
+
+(* Lemma proper_fpr: forall m0 mm, *)
+(*     fpr m0 (same_events_with_stop mm) -> *)
+(*     fstopped m0 = false -> *)
+(*     fpr m0 mm. *)
+(* Proof.  *)
+(*   destruct m0 as [m0 | m0]; induction m0; intros mm Hfpr Hstop; try now auto. *)
+(*   simpl in Hstop. destruct mm; try now auto. *)
+(*   now destruct mm as [mm | mm]. *)
+(* Qed. *)
+
+(* End Embedding'. *)
+
+(* Notation "m '[fstop' es '/ftbd]'" := (same_events_with_stop es m) *)
+(*                                        (at level 50). *)
+
+(* (*******************************************************************************) *)
+
+(* CoInductive t_eq : trace -> trace -> Prop := *)
+(* | estop : forall f, t_eq (tstop f) (tstop f) *)
+(* | esilent : t_eq tsilent tsilent *)
+(* | etrace : forall (e : event) t1 t2, t_eq t1 t2 -> t_eq (tcons e t1) (tcons e t2). *)
+
+(* Lemma t_eq_symm : forall t1 t2, t_eq t1 t2 -> t_eq t2 t1. *)
+(* Proof. *)
+(*   cofix CH. *)
+(*   intros t1 t2 Heq. *)
+(*   inversion Heq; subst; constructor. *)
+(*   now apply CH. *)
+(* Qed. *)
+
+(* Lemma prefix_preserved : forall m t1 t2, prefix m t1 -> t_eq t1 t2 -> prefix m t2. *)
+(* Proof. *)
+(*   intros [m | m]; induction m; intros t1 t2 hpref heq; try now auto. *)
+(*   + destruct t1, t2; try easy. *)
+(*     * inversion hpref; inversion heq; now subst. *)
+(*   + destruct t1, t2; try now auto. inversion hpref. subst.    *)
+(*     inversion heq. subst. simpl. split; try now auto. *)
+(*     now apply (IHm t1 t2). *)
+(*   + destruct t1, t2; try now auto. inversion hpref. subst. *)
+(*     inversion heq. subst. simpl. split; try now auto. *)
+(*     now apply (IHm t1 t2). *)
+(* Qed. *)
+
+(* Lemma same_finite_prefixes : forall t1 t2, t_eq t1 t2 -> *)
+(*                              forall m, (prefix m t1) <-> prefix m t2. *)
+(* Proof. *)
+(*   intros t1 t2 heq m. split; intros H; *)
+(*   [now apply (prefix_preserved m t1 t2) *)
+(*   |apply (prefix_preserved m t2 t1); try now auto]. *)
+(*   now apply t_eq_symm. *)
+(* Qed. *)
+
+(* Lemma neq_finitely_refutable : forall t1 t2, *)
+(*     ~ (t_eq t1 t2) <-> (exists m1 m2, prefix m1 t1 /\ prefix m2 t2 /\ ~ (prefix m1 t2 /\ prefix m2 t1)). *)
+(* Proof. *)
+(*   intros t1 t2. split. *)
+(*   - apply contra. intros H. *)
+(*     rewrite <- dne. *)
+(*     generalize dependent t2. generalize dependent t1. *)
+(*     cofix Hfix. *)
+(*     intros t1 t2 H. *)
+(*     destruct t1 as [| | e1' t1']; destruct t2 as [| | e2' t2']. *)
+(*     + destruct (classic (e = e0)). *)
+(*       * subst; constructor. *)
+(*       * exfalso. apply H. *)
+(*         exists (fstop nil e). exists (fstop nil e0). *)
+(*         repeat split; try now auto. *)
+(*     + exfalso; apply H. *)
+(*       exists (fstop nil e ). exists (ftbd nil). *)
+(*       repeat split; try now auto. *)
+(*     + exfalso; apply H. *)
+(*       exists (fstop nil e). exists (ftbd nil). *)
+(*       repeat split; try now auto. *)
+(*     + exfalso; apply H. *)
+(*       exists (ftbd nil). exists (fstop nil e). *)
+(*       repeat split; try now auto. *)
+(*     + constructor. *)
+(*     + exfalso; apply H. *)
+(*       exists (ftbd nil). exists (ftbd (cons e2' nil)). *)
+(*       repeat split; try now auto. *)
+(*     + exfalso; apply H. *)
+(*       exists (ftbd (cons e1' nil)). exists (fstop nil e). *)
+(*       repeat split; try now auto. *)
+(*     + exfalso; apply H. *)
+(*       exists (ftbd (cons e1' nil)). exists (ftbd nil). *)
+(*       repeat split; try now auto. *)
+(*     + destruct (classic (e1' = e2')). *)
+(*       * subst. specialize (Hfix t1' t2'). *)
+(*         assert (H0: ~(exists m1 m2 : finpref, prefix m1 t1' /\ prefix m2 t2' *)
+(*                                      /\ ~ (prefix m1 t2' /\ prefix m2 t1'))). *)
+(*         { intros Hn. *)
+(*           apply H. destruct Hn as [m1 [m2 [Hm1 [Hm2 Hn]]]]. *)
+(*           destruct m1, m2. *)
+(*           - exists (fstop (cons e2' p) e). exists (fstop (cons e2' p0) e0). *)
+(*             repeat split; try now auto. intros Hn'. *)
+(*             destruct Hn' as [Hn1 Hn2]. *)
+(*             inversion Hn1; inversion Hn2. now auto. *)
+(*           - exists (fstop (cons e2' p) e). exists (ftbd (cons e2' p0)). *)
+(*             repeat split; try now auto. intros Hn'. *)
+(*             destruct Hn' as [Hn1 Hn2]. *)
+(*             inversion Hn1; inversion Hn2. now auto. *)
+(*           - exists (ftbd (cons e2' p)). exists (fstop (cons e2' p0) e). *)
+(*             repeat split; try now auto. intros Hn'. *)
+(*             destruct Hn' as [Hn1 Hn2]. *)
+(*             inversion Hn1; inversion Hn2. now auto. *)
+(*           - exists (ftbd (cons e2' p)). exists (ftbd (cons e2' p0)). *)
+(*             repeat split; try now auto. intros Hn'. *)
+(*             destruct Hn' as [Hn1 Hn2]. *)
+(*             inversion Hn1; inversion Hn2. now auto. *)
+(*         } *)
+(*         specialize (Hfix H0). constructor. assumption. *)
+(*       * exfalso; apply H. *)
+(*         exists (ftbd (cons e1' nil)). exists (ftbd (cons e2' nil)). *)
+(*         repeat split; try now auto. simpl. *)
+(*         intros Hn. *)
+(*         inversion Hn. inversion H1. contradiction. *)
+(*   - intros [m1 [m2 [h1 [h2 hn]]]] hf. apply hn. split. *)
+(*     + now apply (same_finite_prefixes t1 t2). *)
+(*     + apply t_eq_symm in hf. now apply (same_finite_prefixes t2 t1). *)
+(* Qed. *)
+
+(* (*******************************************************************************) *)
+
+(* Definition traces_match (t1 t2 : trace) : Prop := *)
+(*  t1 = t2 \/ *)
+(*  (exists (l : list event) (e1 e2 : event), *)
+(*    is_input e1 /\ is_input e2 /\  e1 <> e2 /\ *)
+(*    prefix (ftbd (snoc l e1)) t1 /\ prefix (ftbd (snoc l e2)) t2). *)
+
+
+(* (* Various lemmas about snoc, fsnoc, and fpr *) *)
+
+Lemma destruct_pref {A : Type} : forall (l : list A),
+    l = nil \/ exists (a : A) (l' : list A),  l = snoc l' a.
 Proof.
-  Print diverges.
-  destruct m as [m f| m]; induction m; intros t Hpref Hembed Hstop Hdiv; try now auto.
-  + destruct t.
-    * specialize (Hembed e). contradiction.
-    * now pose proof div_silent.
-    * now exists e.
-  + destruct t; try now auto.
-    inversion Hpref. subst. destruct (IHm t) as [e' h]; try now auto.
-    * intros ff. specialize (Hembed ff).
-      intros Hembed'.
-      pose proof embed_cons ff (ftbd m) t e as Hcontra. specialize (Hcontra Hembed').
-      now apply Hembed.
-    * intros ff. now pose proof div_cons e t ff.
-    * now exists e'.
-Qed.
-
-Lemma fpr_stop_equal : forall m1 m2,
-    fpr m1 m2 ->
-    fstopped m1 = true ->
-    m1 = m2.
-Proof.
-  intros [m1 | m1]; induction m1; intros [m2 | m2] Hpref Hstop;
-    try easy;
-    inversion Hpref; congruence.
-Qed.
-
-
-(**********************************************************************)
-
-(** *m[fstop/ftbd] *)
-
-Section Embedding'.
-
-Variable es : endstate.
-
-Definition same_events_with_stop (m : finpref) : finpref :=
-  match m with
-  | ftbd m => fstop m es
-  | fstop m f => fstop m f
-  end.
-
-Lemma with_stop_fstopped : forall m,
-    fstopped (same_events_with_stop m) = true.
-Proof. destruct m; auto. Qed.
-
-Lemma if_fstopped_equal : forall m,
-    fstopped m = true ->
-    m = same_events_with_stop m.
-Proof.
-  now destruct m.
-Qed.
-
-Lemma embedding_is_the_same : forall m,
-    embedding es m =
-    embedding es (same_events_with_stop m).
-Proof.
-  intros m. destruct m; try easy.
-Qed.
-
-Lemma m_fpr_with_stop : forall m,
-    fpr m (same_events_with_stop m).
-Proof. destruct m as [m | m]; now induction m. Qed.
-
-Lemma with_stop_prefix_embedding :forall m,
-    prefix (same_events_with_stop m) (embedding es m).
-Proof. destruct m as [m | m]; now induction m. Qed.
-
-Lemma equal_with_stop_same_embedding : forall m mm,
-    fstopped m = true ->
-    fpr mm m ->
-    fpr m (same_events_with_stop mm) ->
-    embedding es m = embedding es mm.
-Proof.
-  destruct m as [m | m]; destruct m;
-    intros mm Hstop Hfpr HfprStop; try now destruct mm.
-  simpl in *. 
-  destruct mm; try now auto; simpl in *. inversion Hfpr; subst. reflexivity.
-  destruct HfprStop; simpl in *; now subst.
-  destruct mm as [mm | mm]; simpl in *;
-    try destruct Hfpr; try destruct HfprStop; now subst.
-Qed.
-
-Lemma proper_fpr: forall m0 mm,
-    fpr m0 (same_events_with_stop mm) ->
-    fstopped m0 = false ->
-    fpr m0 mm.
-Proof. 
-  destruct m0 as [m0 | m0]; induction m0; intros mm Hfpr Hstop; try now auto.
-  simpl in Hstop. destruct mm; try now auto.
-  now destruct mm as [mm | mm].
-Qed.
-
-End Embedding'.
-
-Notation "m '[fstop' es '/ftbd]'" := (same_events_with_stop es m)
-                                       (at level 50).
-
-(*******************************************************************************)
-
-CoInductive t_eq : trace -> trace -> Prop :=
-| estop : forall f, t_eq (tstop f) (tstop f)
-| esilent : t_eq tsilent tsilent
-| etrace : forall (e : event) t1 t2, t_eq t1 t2 -> t_eq (tcons e t1) (tcons e t2).
-
-Lemma t_eq_symm : forall t1 t2, t_eq t1 t2 -> t_eq t2 t1.
-Proof.
-  cofix CH.
-  intros t1 t2 Heq.
-  inversion Heq; subst; constructor.
-  now apply CH.
-Qed.
-
-Lemma prefix_preserved : forall m t1 t2, prefix m t1 -> t_eq t1 t2 -> prefix m t2.
-Proof.
-  intros [m | m]; induction m; intros t1 t2 hpref heq; try now auto.
-  + destruct t1, t2; try easy.
-    * inversion hpref; inversion heq; now subst.
-  + destruct t1, t2; try now auto. inversion hpref. subst.   
-    inversion heq. subst. simpl. split; try now auto.
-    now apply (IHm t1 t2).
-  + destruct t1, t2; try now auto. inversion hpref. subst.
-    inversion heq. subst. simpl. split; try now auto.
-    now apply (IHm t1 t2).
-Qed.
-
-Lemma same_finite_prefixes : forall t1 t2, t_eq t1 t2 ->
-                             forall m, (prefix m t1) <-> prefix m t2.
-Proof.
-  intros t1 t2 heq m. split; intros H;
-  [now apply (prefix_preserved m t1 t2)
-  |apply (prefix_preserved m t2 t1); try now auto].
-  now apply t_eq_symm.
-Qed.
-
-Lemma neq_finitely_refutable : forall t1 t2,
-    ~ (t_eq t1 t2) <-> (exists m1 m2, prefix m1 t1 /\ prefix m2 t2 /\ ~ (prefix m1 t2 /\ prefix m2 t1)).
-Proof.
-  intros t1 t2. split.
-  - apply contra. intros H.
-    rewrite <- dne.
-    generalize dependent t2. generalize dependent t1.
-    cofix Hfix.
-    intros t1 t2 H.
-    destruct t1 as [| | e1' t1']; destruct t2 as [| | e2' t2'].
-    + destruct (classic (e = e0)).
-      * subst; constructor.
-      * exfalso. apply H.
-        exists (fstop nil e). exists (fstop nil e0).
-        repeat split; try now auto.
-    + exfalso; apply H.
-      exists (fstop nil e ). exists (ftbd nil).
-      repeat split; try now auto.
-    + exfalso; apply H.
-      exists (fstop nil e). exists (ftbd nil).
-      repeat split; try now auto.
-    + exfalso; apply H.
-      exists (ftbd nil). exists (fstop nil e).
-      repeat split; try now auto.
-    + constructor.
-    + exfalso; apply H.
-      exists (ftbd nil). exists (ftbd (cons e2' nil)).
-      repeat split; try now auto.
-    + exfalso; apply H.
-      exists (ftbd (cons e1' nil)). exists (fstop nil e).
-      repeat split; try now auto.
-    + exfalso; apply H.
-      exists (ftbd (cons e1' nil)). exists (ftbd nil).
-      repeat split; try now auto.
-    + destruct (classic (e1' = e2')).
-      * subst. specialize (Hfix t1' t2').
-        assert (H0: ~(exists m1 m2 : finpref, prefix m1 t1' /\ prefix m2 t2'
-                                     /\ ~ (prefix m1 t2' /\ prefix m2 t1'))).
-        { intros Hn.
-          apply H. destruct Hn as [m1 [m2 [Hm1 [Hm2 Hn]]]].
-          destruct m1, m2.
-          - exists (fstop (cons e2' p) e). exists (fstop (cons e2' p0) e0).
-            repeat split; try now auto. intros Hn'.
-            destruct Hn' as [Hn1 Hn2].
-            inversion Hn1; inversion Hn2. now auto.
-          - exists (fstop (cons e2' p) e). exists (ftbd (cons e2' p0)).
-            repeat split; try now auto. intros Hn'.
-            destruct Hn' as [Hn1 Hn2].
-            inversion Hn1; inversion Hn2. now auto.
-          - exists (ftbd (cons e2' p)). exists (fstop (cons e2' p0) e).
-            repeat split; try now auto. intros Hn'.
-            destruct Hn' as [Hn1 Hn2].
-            inversion Hn1; inversion Hn2. now auto.
-          - exists (ftbd (cons e2' p)). exists (ftbd (cons e2' p0)).
-            repeat split; try now auto. intros Hn'.
-            destruct Hn' as [Hn1 Hn2].
-            inversion Hn1; inversion Hn2. now auto.
-        }
-        specialize (Hfix H0). constructor. assumption.
-      * exfalso; apply H.
-        exists (ftbd (cons e1' nil)). exists (ftbd (cons e2' nil)).
-        repeat split; try now auto. simpl.
-        intros Hn.
-        inversion Hn. inversion H1. contradiction.
-  - intros [m1 [m2 [h1 [h2 hn]]]] hf. apply hn. split.
-    + now apply (same_finite_prefixes t1 t2).
-    + apply t_eq_symm in hf. now apply (same_finite_prefixes t2 t1).
-Qed.
-
-(*******************************************************************************)
-
-Axiom is_input : event -> Prop.
-
-Definition traces_match (t1 t2 : trace) : Prop := 
- t1 = t2 \/
- (exists (m : finpref) (e1 e2 : event),
-   is_input e1 /\ is_input e2 /\  e1 <> e2 /\
-   fstopped m = false /\ prefix (fsnoc m e1) t1 /\ prefix (fsnoc m e2) t2).
-
-
-(* Various lemmas about snoc, fsnoc, and fpr *)
-
-Lemma destruct_pref : forall (m : pref), m = nil \/ exists (e : event) (m' : pref),  m = snoc m' e.
-Proof.
-  induction m.
+  induction l. 
   - now left.
-  - right. destruct IHm.
+  - right. destruct IHl.
     + subst. now exists a, nil.
     + destruct H as [e [m' H]]. subst.
       now exists e, (cons a m').
 Qed.
 
-Lemma snoc_length : forall (m' : pref) (e : event) (n : nat),
-    Datatypes.length (snoc m' e) = S n -> Datatypes.length m' = n.
+Lemma snoc_length {A : Type} : forall (l' : list A) (a : A) (n : nat),
+    Datatypes.length (snoc l' a) = S n -> Datatypes.length l' = n.
 Proof.
-  induction m'.
+  induction l'.
   - intros. simpl in H. inversion H. reflexivity.
   - intros e n Hlen. simpl in *. inversion Hlen.
     destruct n as [| m].
-    + destruct m'; now auto.
-    + specialize (IHm' e m H0). now subst.
+    + destruct l'; now auto.
+    + rewrite H0. now rewrite (IHl' e m).  
 Qed.
 
-Definition length (m : finpref) :=
-  match m with
-  | fstop m _ => Datatypes.length m
-  | ftbd  m => Datatypes.length m
-  end.
+(* Definition length (m : finpref) := *)
+(*   match m with *)
+(*   | fstop m _ => Datatypes.length m *)
+(*   | ftbd  m => Datatypes.length m *)
+(*   end. *)
 
-Theorem finpref_ind_snoc :
-  forall (P : finpref -> Prop),
-    P (ftbd nil) ->
-    (forall (m : pref) (f : endstate), P (fstop m f)) ->
-    (forall (m : finpref) (e : event), P m -> P (fsnoc m e)) ->
-    forall m, P m.
-Proof.
-  intros P Hnil Hstop Hind.
-  assert (H: forall (n : nat) (m : finpref), length m = n -> P m).
-  { induction n.
-    - intros [m f | m] Hlen; try now auto.
-      destruct m; try now auto.
-    - intros m Hlen.
-      destruct m; try now auto.
-      destruct (destruct_pref p).
-      subst; simpl in *. inversion Hlen.
-      destruct H as [e' [p' H']].
-      subst; apply snoc_length in Hlen. specialize (IHn (ftbd p') Hlen).
-      now specialize (Hind (ftbd p') e' (IHn)).
-  }
-  intros m. now apply (H (length m) m).
-Qed.
+(* Theorem finpref_ind_snoc : *)
+(*   forall (P : finpref -> Prop), *)
+(*     P (ftbd nil) -> *)
+(*     (forall (m : pref) (f : endstate), P (fstop m f)) -> *)
+(*     (forall (m : finpref) (e : event), P m -> P (fsnoc m e)) -> *)
+(*     forall m, P m. *)
+(* Proof. *)
+(*   intros P Hnil Hstop Hind. *)
+(*   assert (H: forall (n : nat) (m : finpref), length m = n -> P m). *)
+(*   { induction n. *)
+(*     - intros [m f | m] Hlen; try now auto. *)
+(*       destruct m; try now auto. *)
+(*     - intros m Hlen. *)
+(*       destruct m; try now auto. *)
+(*       destruct (destruct_pref p). *)
+(*       subst; simpl in *. inversion Hlen. *)
+(*       destruct H as [e' [p' H']]. *)
+(*       subst; apply snoc_length in Hlen. specialize (IHn (ftbd p') Hlen). *)
+(*       now specialize (Hind (ftbd p') e' (IHn)). *)
+(*   } *)
+(*   intros m. now apply (H (length m) m). *)
+(* Qed. *)
 
-Theorem pref_ind_snoc :
-  forall (P : pref -> Prop),
+Theorem list_ind_snoc {A : Type} :
+  forall (P : list A -> Prop),
     P nil ->
-    (forall (p : pref) (e : event), P p -> P (snoc p e)) ->
-    forall p, P p.
+    (forall (l : list A) (a : A), P l -> P (snoc l a)) ->
+    forall l, P l.
 Proof.
   intros P Hnil Hind.
-  assert (H: forall (n : nat) (p : pref), Datatypes.length p = n -> P p).
+  assert (H: forall (n : nat) (l : list A), Datatypes.length l = n -> P l).
   { induction n.
-    - intros p Hlen; try now auto.
-      destruct p; try now auto.
-    - intros p Hlen.
-      destruct (destruct_pref p); try now auto.
+    - intros l Hlen; try now auto.
+      destruct l; try now auto.
+    - intros l Hlen.
+      destruct (destruct_pref l); try now auto.
       subst; assumption.
       destruct H as [e' [p' H']].
       subst; apply snoc_length in Hlen. specialize (IHn p' Hlen).
@@ -982,112 +992,112 @@ Proof.
   intros p. now apply (H (Datatypes.length p) p).
 Qed.
 
-Lemma snoc_injective : forall (e1 e2 : event) p1 p2,
-  snoc p1 e1 = snoc p2 e2 -> e1 = e2 /\ p1 = p2.
-Proof.
-  intros e1 e2. induction p1.
-  - intros p2 H; destruct p2; inversion H; try now auto.
-    destruct p2; try now auto.
-  - intros p2 H. simpl in *. destruct p2; try now auto.
-    inversion H. subst. simpl in *. destruct p1; try now auto.
-    simpl in *. inversion H.
-    specialize (IHp1 p2 H2). destruct IHp1 as [Heq Heq'].
-    split. assumption. now subst.
-Qed.
+(* Lemma snoc_injective : forall (e1 e2 : event) p1 p2, *)
+(*   snoc p1 e1 = snoc p2 e2 -> e1 = e2 /\ p1 = p2. *)
+(* Proof. *)
+(*   intros e1 e2. induction p1. *)
+(*   - intros p2 H; destruct p2; inversion H; try now auto. *)
+(*     destruct p2; try now auto. *)
+(*   - intros p2 H. simpl in *. destruct p2; try now auto. *)
+(*     inversion H. subst. simpl in *. destruct p1; try now auto. *)
+(*     simpl in *. inversion H. *)
+(*     specialize (IHp1 p2 H2). destruct IHp1 as [Heq Heq']. *)
+(*     split. assumption. now subst. *)
+(* Qed. *)
 
-Lemma destruct_fpr_ftbd_snoc : forall p' p e,
-  fpr_ftbd p' (snoc p e) ->
-  p' = snoc p e \/ fpr_ftbd p' p.
-Proof.
-  induction p' as [| e' p''].
-  - intros p e H. simpl in *. tauto.
-  - intros p e H. simpl in H.
-    remember (snoc p e) as pe. destruct pe as [| e'' p''']. tauto.
-    destruct H as [H1 H2]. subst e''.
-    destruct (destruct_pref p''') as [| [e''' [p'''' H]]].
-    + subst p'''. destruct p as [| e1 [| e2 ]]; simpl in Heqpe.
-      * destruct p''. now left. simpl in H2; tauto.
-      * now inversion Heqpe.
-      * now inversion Heqpe.
-    + subst p'''. destruct (IHp'' _ _ H2) as [IH | IH].
-      * subst p''. left. reflexivity.
-      * destruct p as [| e1 [| e2 ]]; simpl in Heqpe.
-        ++ destruct p''''; simpl in *; now inversion Heqpe.
-        ++ inversion Heqpe. destruct p''''; simpl in *.
-           -- right. tauto.
-           -- inversion H1. subst. destruct p''''; simpl in *; now inversion Heqpe.
-        ++ inversion Heqpe. subst e1. right. simpl. split. reflexivity.
-           replace (e2 :: snoc l e) with (snoc (e2 :: l) e) in H1 by reflexivity.
-           apply snoc_injective in H1. destruct H1 as [H11 H12]. now subst.
-Qed.
+(* Lemma destruct_fpr_ftbd_snoc : forall p' p e, *)
+(*   fpr_ftbd p' (snoc p e) -> *)
+(*   p' = snoc p e \/ fpr_ftbd p' p. *)
+(* Proof. *)
+(*   induction p' as [| e' p'']. *)
+(*   - intros p e H. simpl in *. tauto. *)
+(*   - intros p e H. simpl in H. *)
+(*     remember (snoc p e) as pe. destruct pe as [| e'' p''']. tauto. *)
+(*     destruct H as [H1 H2]. subst e''. *)
+(*     destruct (destruct_pref p''') as [| [e''' [p'''' H]]]. *)
+(*     + subst p'''. destruct p as [| e1 [| e2 ]]; simpl in Heqpe. *)
+(*       * destruct p''. now left. simpl in H2; tauto. *)
+(*       * now inversion Heqpe. *)
+(*       * now inversion Heqpe. *)
+(*     + subst p'''. destruct (IHp'' _ _ H2) as [IH | IH]. *)
+(*       * subst p''. left. reflexivity. *)
+(*       * destruct p as [| e1 [| e2 ]]; simpl in Heqpe. *)
+(*         ++ destruct p''''; simpl in *; now inversion Heqpe. *)
+(*         ++ inversion Heqpe. destruct p''''; simpl in *. *)
+(*            -- right. tauto. *)
+(*            -- inversion H1. subst. destruct p''''; simpl in *; now inversion Heqpe. *)
+(*         ++ inversion Heqpe. subst e1. right. simpl. split. reflexivity. *)
+(*            replace (e2 :: snoc l e) with (snoc (e2 :: l) e) in H1 by reflexivity. *)
+(*            apply snoc_injective in H1. destruct H1 as [H11 H12]. now subst. *)
+(* Qed. *)
 
 
-(* Axiom tapp : finpref -> trace -> trace. *) (* Where have all the flowers gone? *)
+(* (* Axiom tapp : finpref -> trace -> trace. *) (* Where have all the flowers gone? *) *)
 
-Fixpoint tapp' (p : pref) (t : trace) : trace :=
-  match p with
-  | nil => t
-  | cons e p' => tcons e (tapp' p' t)
-  end.
+(* Fixpoint tapp' (p : pref) (t : trace) : trace := *)
+(*   match p with *)
+(*   | nil => t *)
+(*   | cons e p' => tcons e (tapp' p' t) *)
+(*   end. *)
 
-Definition tapp (m : finpref) (t : trace) : trace :=
-  match m with
-  | fstop p f => embedding f (fstop p f) (* justification:
-                           we can't really add anything after a stopped trace. *)
-  | ftbd  p => tapp' p t
-  end.
+(* Definition tapp (m : finpref) (t : trace) : trace := *)
+(*   match m with *)
+(*   | fstop p f => embedding f (fstop p f) (* justification: *)
+(*                            we can't really add anything after a stopped trace. *) *)
+(*   | ftbd  p => tapp' p t *)
+(*   end. *)
 
-Lemma tapp_pref : forall (m : finpref) (t : trace),
-    prefix m (tapp m t).
-Proof.
-  induction finpref m as e f p IHp; intros; try now auto;
-    split; simpl in *; now auto.
-Qed.
+(* Lemma tapp_pref : forall (m : finpref) (t : trace), *)
+(*     prefix m (tapp m t). *)
+(* Proof. *)
+(*   induction finpref m as e f p IHp; intros; try now auto; *)
+(*     split; simpl in *; now auto. *)
+(* Qed. *)
 
-Lemma tapp_div_pref : forall (t : trace),
-    diverges t -> exists (m : finpref), fstopped m = false /\ t = tapp m tsilent.
-Proof.
-  intros t Ht.
-  induction Ht.
-  - now (exists (ftbd nil)).
-  - destruct IHHt as [m Hm].
-    destruct m as [p f | p].
-    + now destruct Hm.
-    + destruct Hm as [H1 H2].
-      exists ((ftbd (cons e p))).
-      split; now subst.
-Qed.
+(* Lemma tapp_div_pref : forall (t : trace), *)
+(*     diverges t -> exists (m : finpref), fstopped m = false /\ t = tapp m tsilent. *)
+(* Proof. *)
+(*   intros t Ht. *)
+(*   induction Ht. *)
+(*   - now (exists (ftbd nil)). *)
+(*   - destruct IHHt as [m Hm]. *)
+(*     destruct m as [p f | p]. *)
+(*     + now destruct Hm. *)
+(*     + destruct Hm as [H1 H2]. *)
+(*       exists ((ftbd (cons e p))). *)
+(*       split; now subst. *)
+(* Qed. *)
 
-Lemma tapp_fin_pref : forall (t : trace),
-    fin t -> exists (m : finpref) (f : endstate), t = tapp m (tstop f).
-Proof.
-  intros t Ht.
-  induction Ht.
-  - exists (fstop nil f), f. reflexivity.
-  - destruct IHHt as [m [f Hm]].
-    destruct m as [p f' | p]; subst.
-    + exists (fstop (cons e p) f'), f'. reflexivity.
-    + exists (ftbd (cons e p)), f. simpl in *. reflexivity.
-Qed.
+(* Lemma tapp_fin_pref : forall (t : trace), *)
+(*     fin t -> exists (m : finpref) (f : endstate), t = tapp m (tstop f). *)
+(* Proof. *)
+(*   intros t Ht. *)
+(*   induction Ht. *)
+(*   - exists (fstop nil f), f. reflexivity. *)
+(*   - destruct IHHt as [m [f Hm]]. *)
+(*     destruct m as [p f' | p]; subst. *)
+(*     + exists (fstop (cons e p) f'), f'. reflexivity. *)
+(*     + exists (ftbd (cons e p)), f. simpl in *. reflexivity. *)
+(* Qed. *)
 
-Lemma pref_inf_ndiv_pref : forall (m : finpref) (t : trace),
-  prefix m t -> inf t -> ~diverges t -> exists e, prefix (fsnoc m e) t.
-Proof.
-  induction finpref m as e f p IHp; intros t H H0 H1; try now eauto.
-  - destruct t; try now auto.
-    + exfalso; apply H0. now constructor.
-    + exfalso; apply H1. now constructor.
-    + now (exists e).
-  - destruct t; try now auto.
-    simpl in *. destruct H; subst.
-    specialize (IHp t H2 (inf_tcons e0 t H0)).
-    assert (~ diverges (tcons e0 t) -> ~ diverges t).
-    { clear.
-      destruct t; try now auto.
-      - intros H. exfalso. apply H. constructor. constructor.
-      - intros H. intros H'. apply H. now constructor. }
-    specialize (IHp (H H1)).
-    destruct IHp as [e He]. now (exists e).
-  Unshelve.
-  exact an_event. exact an_event.
-Qed.
+(* Lemma pref_inf_ndiv_pref : forall (m : finpref) (t : trace), *)
+(*   prefix m t -> inf t -> ~diverges t -> exists e, prefix (fsnoc m e) t. *)
+(* Proof. *)
+(*   induction finpref m as e f p IHp; intros t H H0 H1; try now eauto. *)
+(*   - destruct t; try now auto. *)
+(*     + exfalso; apply H0. now constructor. *)
+(*     + exfalso; apply H1. now constructor. *)
+(*     + now (exists e). *)
+(*   - destruct t; try now auto. *)
+(*     simpl in *. destruct H; subst. *)
+(*     specialize (IHp t H2 (inf_tcons e0 t H0)). *)
+(*     assert (~ diverges (tcons e0 t) -> ~ diverges t). *)
+(*     { clear. *)
+(*       destruct t; try now auto. *)
+(*       - intros H. exfalso. apply H. constructor. constructor. *)
+(*       - intros H. intros H'. apply H. now constructor. } *)
+(*     specialize (IHp (H H1)). *)
+(*     destruct IHp as [e He]. now (exists e). *)
+(*   Unshelve. *)
+(*   exact an_event. exact an_event. *)
+(* Qed. *)
