XPrefix.v
@@ -4,45 +4,42 @@ Require Import Setoid.
 Require Import List.
 Require Import TraceModel.
 
-Inductive xpref : Set :=
-| xstop : pref -> endstate -> xpref
-| xtbd  : pref -> xpref
-| xsilent : pref -> xpref.
+Variant xpref : Set :=
+| xstop   (l : list event) (e : endstate) : xpref
+| xtbd    (l : list event)                : xpref
+| xsilent (l : list event)                : xpref. 
+
 
 (** Prefix relation between extended prefixes and traces *)
 
-Fixpoint xsilent_prefix (m : pref) (t : trace) : Prop :=
-  match m, t with
-    | nil, tsilent => True
-    | nil, _        => False
-    | cons e1 m', tcons e2 t' => e1 = e2 /\ xsilent_prefix m' t'
-    | _, _          => False
-  end.
+Definition xprefix (x : xpref) (t : trace) : Prop :=
+ match x, t with
+ | xstop   lx ex, tstop lt et => ex = et /\ lx = lt
+ | xsilent lx   , tsilent lt   => lx = lt
+ | xtbd    lx   , tstop lt et => list_list_prefix lx lt
+ | xtbd    lx   , tsilent lt  => list_list_prefix lx lt
+ | xtbd    lx   , tstream s   => list_stream_prefix lx s
+ | _, _ => False
+ end. 
 
-Definition xprefix (m : xpref) (t : trace) : Prop :=
-  match m with
-  | xstop m f => fstop_prefix m f t
-  | xtbd m  => ftbd_prefix m t
-  | xsilent m => xsilent_prefix m t
-  end.
 
 Definition xembed (m:finpref) : xpref :=
   match m with
-  | fstop m f => xstop m f
-  | ftbd m  => xtbd m
+  | fstop l f => xstop l f
+  | ftbd  l   => xtbd l
   end.
 
-Lemma xsilent_prefix_ftbd_prefix : forall p t,
-  xsilent_prefix p t -> ftbd_prefix p t.
-Proof.
-  induction p; destruct t; simpl; try tauto. intros [H1 H2]. subst a. eauto.
-Qed.
+(* Lemma xsilent_prefix_ftbd_prefix : forall p t, *)
+(*   xsilent_prefix p t -> ftbd_prefix p t. *)
+(* Proof. *)
+(*   induction p; destruct t; simpl; try tauto. intros [H1 H2]. subst a. eauto. *)
+(* Qed. *)
 
 Lemma prefix_xprefix_xembed : forall m t, prefix m t -> xprefix (xembed m) t.
-Proof. intros m t H. destruct m; simpl in *; assumption. Qed.
+Proof. intros [] []; auto.  Qed.
 
 Lemma xprefix_xembed_prefix : forall m t, xprefix (xembed m) t -> prefix m t.
-Proof. intros m t H. destruct m; simpl in *; assumption. Qed.
+Proof. intros [] []; auto.  Qed.
 
 (* Also definitions corresponding to CommonST *)
 
