Events.v
@@ -9,4 +9,9 @@ Axiom event : Set.
 Axiom an_event : event.
 Axiom another_event : event.
 Axiom different_events : an_event <> another_event.
-Axiom eq_event_dec : forall (e1 e2 : event), {e1 = e2} + {e1 <> e2}.
+Axiom eq_event_dec : forall (e1 e2 : event), {e1 = e2} + {e1 <> e2}. 
+
+Axiom endstate : Set.
+Axiom an_endstate : endstate.
+
+Axiom is_input : event -> Prop.
